Rename [Det]Automata to [Det]Autonmaton

AutomataTheory/AutomataBasic.lean
@@ -12,42 +12,42 @@ open BigOperators Function Set Filter
 
 section AutomataBasic
 
-class Automata (A : Type*) where
+class Automaton (A : Type*) where
   State : Type*
   init : Set State
   next : State → A → Set State
 
 variable {A : Type*}
 
-def FinRun (M : Automata A) (n : ℕ) (as : Fin n → A) (ss : Fin (n + 1) → M.State) :=
+def FinRun (M : Automaton A) (n : ℕ) (as : Fin n → A) (ss : Fin (n + 1) → M.State) :=
   ss 0 ∈ M.init ∧ ∀ k : Fin n, ss (k + 1) ∈ M.next (ss k) (as k)
 
-def OptFinRun (M : Automata A) (n : ℕ) (as' : ℕ → Option A) (ss' : ℕ → Option M.State) :=
+def OptFinRun (M : Automaton A) (n : ℕ) (as' : ℕ → Option A) (ss' : ℕ → Option M.State) :=
   (∃ s0 ∈ M.init, ss' 0 = some s0) ∧
   (∀ k < n, ∃ sk ak sk_1, sk_1 ∈ M.next sk ak ∧ ss' k = some sk ∧ as' k = some ak ∧ ss' (k + 1) = some sk_1)
 
-def InfRun (M : Automata A) (as : ℕ → A) (ss : ℕ → M.State) :=
+def InfRun (M : Automaton A) (as : ℕ → A) (ss : ℕ → M.State) :=
   ss 0 ∈ M.init ∧ ∀ k : ℕ, ss (k + 1) ∈ M.next (ss k) (as k)
 
-def FinAccept (M : Automata A) (acc : Set M.State) (n : ℕ) (as : Fin n → A) :=
+def FinAccept (M : Automaton A) (acc : Set M.State) (n : ℕ) (as : Fin n → A) :=
   ∃ ss : Fin (n + 1) → M.State, FinRun M n as ss ∧ ss n ∈ acc
 
-def BuchiAccept (M : Automata A) (acc : Set M.State) (as : ℕ → A) :=
+def BuchiAccept (M : Automaton A) (acc : Set M.State) (as : ℕ → A) :=
   ∃ ss : ℕ → M.State, InfRun M as ss ∧ ∃ᶠ k in atTop, ss k ∈ acc
 
-def MullerAccept (M : Automata A) (accSet : Set (Set M.State)) (as : ℕ → A) :=
+def MullerAccept (M : Automaton A) (accSet : Set (Set M.State)) (as : ℕ → A) :=
   ∃ ss : ℕ → M.State, InfRun M as ss ∧ ∃ acc ∈ accSet, ∀ s, s ∈ acc ↔ (∃ᶠ k in atTop, ss k = s)
 
-def RabinAccept (M : Automata A) (accPairs : Set (Set M.State × Set M.State)) (as : ℕ → A) :=
+def RabinAccept (M : Automaton A) (accPairs : Set (Set M.State × Set M.State)) (as : ℕ → A) :=
   ∃ ss : ℕ → M.State, InfRun M as ss ∧ ∃ pair ∈ accPairs, (∃ᶠ k in atTop, ss k ∈ pair.1) ∧ (∀ᶠ k in atTop, ss k ∉ pair.2)
 
-def StreettAccept (M : Automata A) (accPairs : Set (Set M.State × Set M.State)) (as : ℕ → A) :=
+def StreettAccept (M : Automaton A) (accPairs : Set (Set M.State × Set M.State)) (as : ℕ → A) :=
   ∃ ss : ℕ → M.State, InfRun M as ss ∧ ∀ pair ∈ accPairs, (∃ᶠ k in atTop, ss k ∈ pair.1) → (∃ᶠ k in atTop, ss k ∈ pair.2)
 
-def AcceptedLang (M : Automata A) (acc : Set M.State) : Set (List A) :=
+def AcceptedLang (M : Automaton A) (acc : Set M.State) : Set (List A) :=
   { al | ∃ n as, FinAccept M acc n as ∧ al = List.ofFn as }
 
-def AcceptedOmegaLang (M : Automata A) (acc : Set M.State) : Set (ℕ → A) :=
+def AcceptedOmegaLang (M : Automaton A) (acc : Set M.State) : Set (ℕ → A) :=
   { as | BuchiAccept M acc as }
 
 end AutomataBasic
